restructure indicies computations

crypto_examples/ntt.dfy
@@ -53,76 +53,32 @@ module ntt {
         }
     }
 
-    predicate n_sized_diff_chunk(y1: n_sized, y2: n_sized, len: pow2_t, ki: nat)
+    function read_chunk(y: n_sized, len: pow2_t, ki: nat): seq<elem>
         requires 0 <= len.exp <= L;
         requires ki < chunk_count(len);
+        ensures 0 <= ki * len.full <= N - len.full;
     {
-        var offset := ki * len.full;
         chunk_index_bounded(len, ki);
-        forall i | (0 <= i < offset || offset + len.full <= i < N) :: 
-            y1[i] == y2[i]
+        y[ki * len.full..ki * len.full + len.full]
     }
 
-    function view_as_chunks(y: n_sized, len: pow2_t): seq<seq<elem>>
+    function y_as_chunks(y: n_sized, len: pow2_t): (cs: seq<seq<elem>>)
         requires 0 <= len.exp <= L;
     {
         var max_count := chunk_count(len);
-        var csize := len.full;
-        chunk_index_bounded_auto(len);
-        seq(max_count, ki requires 0 <= ki < max_count => y[ki * csize..ki * csize + csize])
+        seq(max_count, ki requires 0 <= ki < max_count => read_chunk(y, len, ki))
     }
 
-    lemma n_sized_diff_chunk_view(y1: n_sized, y2: n_sized, len: pow2_t, ki: nat)
+    lemma y_as_chunks_index_lemma(y: n_sized, len: pow2_t, ki: nat)
         requires 0 <= len.exp <= L;
         requires ki < chunk_count(len);
-        requires n_sized_diff_chunk(y1, y2, len, ki);
-        ensures view_as_chunks(y2, len) ==
-            view_as_chunks(y1, len)[ki := view_as_chunks(y2, len)[ki]]
+        ensures y_as_chunks(y, len)[ki] == read_chunk(y, len, ki);
     {
-        var v1 := view_as_chunks(y1, len);
-        var v2 := view_as_chunks(y2, len);
-        chunk_index_bounded_auto(len);
-        var csize := len.full;
-
-        forall i | 0 <= i < chunk_count(len)
-            ensures i != ki ==> v1[i] == v2[i];
-        {
-            if i != ki {
-                var lo := i * csize;
-                var hi := i * csize + csize;
-                assume y1[lo..hi] == y2[lo..hi]; // TODO
-                assert v1[i] == v2[i];
-            }
-        }
-        assert v2 == v1[ki := v2[ki]];
-    }
-
-    function {:opaque} view_as_chunks_prefix(y: n_sized, len: pow2_t, i: nat): seq<seq<elem>>
-        requires 0 <= len.exp <= L;
-        requires i <= chunk_count(len);
-    {
-        var max_count := chunk_count(len);
-        var count := i;
-        var csize := len.full;
-        chunk_index_bounded_auto(len);
-        seq(count, ki requires 0 <= ki < count => y[ki * csize..ki * csize + csize])    
-    }
-
-    function {:opaque} view_as_chunks_suffix(y: n_sized, len: pow2_t, i: nat): seq<seq<elem>>
-        requires 0 <= len.exp <= L;
-        requires i <= chunk_count(len);
-    {
-        var max_count := chunk_count(len);
-        var count := max_count - i;
-        var csize := len.full;
-        chunk_index_bounded_auto(len);
-        seq(count, ki requires 0 <= ki < count => y[ki * csize..ki * csize + csize]) 
     }
 
     datatype ntt_loop_lvls = ntt_loop_lvls(
         lower: level_view,
-        higher: level_view,
-        ki: nat)
+        higher: level_view)
     {
         predicate ntt_loop_views_wf()
         {
@@ -130,114 +86,212 @@ module ntt {
             && 2 <= higher.m.full <= N
             && 1 <= higher.m.exp <= L
             && lower.m == pow2_half(higher.m)
-            && ki <= chunk_count(higher.m)
             && lower.valid_level_view()
             && higher.valid_level_view()
         }
 
-        function lower_idx(): (i: nat)
+        function lo_idx(ki: nat): (i: nat)
             requires ntt_loop_views_wf();
+            requires ki <= chunk_count(higher.m)
             ensures i <= chunk_count(lower.m);
         {
             chunk_count_half(higher.m);
             ki * 2
         }
 
-        function higher_idx(): nat
+        function hi_idx(ki: nat): nat
+            requires ntt_loop_views_wf();
+            requires ki <= chunk_count(higher.m);
         {
             ki
         }
 
-        function lower_suffix(): seq<seq<elem>>
-            requires ntt_loop_views_wf()
-        {
-            lower.ntt_rec3()[..lower_idx()]
-        }
-
-        function higher_prefix(): seq<seq<elem>>
-            requires ntt_loop_views_wf()
-        {
-            higher.ntt_rec3()[higher_idx()..]
-        }
-
-        lemma index_bounded_lemma(
-            j: nat)
+        lemma hi_lo_idx_relations(ki: nat)
             requires ntt_loop_views_wf();
-            requires 0 <= j < lower.m.full;
+            requires ki <= chunk_count(higher.m);
+            ensures  0 <= lo_idx(ki) * lower.m.full == hi_idx(ki) * higher.m.full;
+            ensures hi_idx(ki) < chunk_count(higher.m) ==> 
+                lo_idx(ki) < chunk_count(lower.m) - 1;
+        {
+            calc == {
+                hi_idx(ki) * higher.m.full;
+                {
+                    LemmaMulIsAssociativeAuto();
+                }
+                ki * 2 * lower.m.full;
+                {
+                    LemmaMulIsAssociativeAuto();
+                }
+                lo_idx(ki) * lower.m.full;
+            }
+
+            if hi_idx(ki) < chunk_count(higher.m) {
+                chunk_count_half(higher.m);
+                assert chunk_count(higher.m) * 2 == chunk_count(lower.m);
+                assert ki <= chunk_count(higher.m) - 1;
+                assert ki * 2 <= (chunk_count(higher.m) - 1) * 2;
+                assert lo_idx(ki) < chunk_count(lower.m) - 1;
+            }
+
+            LemmaMulNonnegative(lo_idx(ki), lower.m.full);
+        }
+
+        lemma index_bounded_lemma(ki: nat, j: nat)
+            requires ntt_loop_views_wf();
+            requires ki <= chunk_count(higher.m);
+            requires 0 <= j <= lower.m.full;
             requires ki < chunk_count(higher.m);
-            ensures 0 <= ki * higher.m.full + j + lower.m.full < N;
+            ensures j != lower.m.full ==>
+                0 <= ki * higher.m.full + j + lower.m.full < N;
+            ensures j == lower.m.full ==>
+                0 <= ki * higher.m.full + j + lower.m.full <= N;
         {
             var len := higher.m.full;
             chunk_index_bounded(higher.m, ki);
             assert 0 <= ki * len <= N - len;
         }
-    }
-    
-    predicate ntt_chunk_loop_inv(
-        y: seq<elem>,
-        view: ntt_loop_lvls)
-    {
-        && view.ntt_loop_views_wf()
-        && |y| == N == pow2(L).full
-        && view_as_chunks_suffix(y, view.lower.m, view.lower_idx())
-            == view.lower_suffix()
-        && view_as_chunks_prefix(y, view.higher.m, view.higher_idx())
-            == view.higher_prefix()
-    }
 
-    method ntt_chunk_loop(
-        y: seq<elem>, 
-        k: nat,
-        view: ntt_loop_lvls)
-    returns (y': seq<elem>)
-        requires ntt_chunk_loop_inv(y, view);
-        requires view.ki < chunk_count(view.higher.m);
-        requires k == view.higher_idx() * view.higher.m.full;
-    {
-        y' := y;
-        var len' := view.lower.m;
-        var omgm := omega_n(view.higher.m);
-
-        var omg := 1;
-        var j := 0;
-
-        assert omg == modpow(omgm, 0) by {
-            LemmaPow0Auto();
-        }
-
-        pow2_basics(view.higher.m);
-
-        view.index_bounded_lemma(0);
-
-        while (j < len'.full)
-            invariant 0 <= j <= len'.full;
-            invariant omg == modpow(omgm, j);
-            invariant |y'| == |y|;
-            invariant k + j + len'.full <= N;
-            invariant y[..k] == y'[..k];
-            invariant y[k+j..k+len'.full] == y'[k+j..k+len'.full];
-            invariant y[k+len'.full+j..] == y'[k+len'.full+j..];
+        function hi_idx_as_glb_offset(ki: nat): (k: nat)
+            requires ntt_loop_views_wf();
+            requires ki < chunk_count(higher.m);
+            ensures k == hi_idx(ki) * higher.m.full;
+            ensures 0 <= k <= N - lower.m.full;
         {
-            view.index_bounded_lemma(j);
-
-            var t := modmul(omg, y[k + j + len'.full]);
-            var u := y[k + j];
-            y' := y'[k + j := modadd(u, t)];
-            y' := y'[k + j + len'.full := modsub(u, t)];
-
-            omg_inv(omgm, omg, view.higher.m, j);
-            omg := modmul(omg, omgm);
-            j := j + 1;
-
-            // if m.exp == 1 {
-            //    ghost var y_exp := ntt_rec2_base(a[ki], m, idxs[ki], ki);
-            //    assert y'[k..k+2] == y_exp; 
-            // }
+            hi_lo_idx_relations(ki);
+            chunk_index_bounded(lower.m, lo_idx(ki));
+            lo_idx(ki) * lower.m.full
         }
 
-    // //     // assert y[..k] == y'[..k];
-    // //     // assert y[k+m.full..] == y'[k+m.full..];
+        predicate ntt_level_loop_inv(y: n_sized, ki: nat)
+        {
+            && ntt_loop_views_wf()
+            && ki <= chunk_count(higher.m)
+            && |y| == N == pow2(L).full
+            && y_as_chunks(y, lower.m)[lo_idx(ki)..]
+                == lower.ntt_rec3()[lo_idx(ki)..]
+            // && y_as_chunks(y, higher.m)[..hi_idx(ki)]
+            //     == higher_prefix()
+        }
+
+        lemma lower_view_correspondence(y: n_sized, ki: nat)
+            requires ntt_level_loop_inv(y, ki);
+            requires hi_idx(ki) < chunk_count(higher.m);
+            ensures lo_idx(ki) < |lower.a| - 1;
+            ensures poly_eval_all_points(lower.a[lo_idx(ki)], read_chunk(y, lower.m, lo_idx(ki)), lower.m);
+            ensures poly_eval_all_points(lower.a[lo_idx(ki)+1], read_chunk(y, lower.m, lo_idx(ki)+1), lower.m);
+        {
+            var k := hi_idx_as_glb_offset(ki);
+            var len' := lower.m;
+            var csize := len'.full;
+            index_bounded_lemma(ki, csize);
+            var even_chunk := y[k..k+csize];
+            var odd_chunk := y[k+csize..k+csize*2];
+            var gy := y_as_chunks(y, lower.m);
+            var vy := lower.ntt_rec3();
+
+            var kl := lo_idx(ki);
+            assert gy[kl..] == vy[kl..];
+
+            hi_lo_idx_relations(ki);
+            assert k == kl * csize;
+            calc == {
+                odd_chunk;
+                y[kl*csize+csize..kl*csize+2*csize];
+                {
+                    LemmaMulIsDistributiveAddOtherWayAuto();
+                }
+                y[(kl+1) * csize..kl*csize+csize+csize];
+                {
+                    LemmaMulIsDistributiveAddOtherWayAuto();
+                }
+                y[(kl+1) * csize..(kl+1) * csize+csize];
+                read_chunk(y, len', kl + 1);
+            }
+            assert even_chunk == read_chunk(y, len', kl);
+            assert odd_chunk == read_chunk(y, len', kl + 1);
+
+            assert even_chunk == vy[kl];
+            assert odd_chunk == vy[kl + 1];
+        }
+
+        // function method even_lo(): (elo: nat)
+        //     ensures elo == lo_idx() * lower.m.full
+        //     ensures 
+        // {
+        //     hi_lo_idx_relations();
+        //     hi_idx() * higher.m.full
+        // }
+
+        // function method even_hi(): (ehi: nat)
+        //     ensures ehi == lo_idx() * lower.m.full + lower.m.full
+        // {
+        //     even_lo() + lower.m.full
+        // }
+
+        // predicate ntt_chunk_loop_inv(y: n_sized, y': n_sized, , ki: nat, j: nat)
+        // {
+        //     && ntt_level_loop_inv(y, ki)
+        //     // && y'[k+j..k+len'.full] == y[k+j..k+len'.full] == read_chunk(y, view.lower.m, view.lo_idx())[j..]
+        //     // && y'[k+len'.full+j..k+len'.full * 2] == y[k+len'.full+j..k+len'.full * 2] == 
+        // }
     }
+
+    // method ntt_chunk_loop(
+    //     y: n_sized, 
+    //     k: nat,
+    //     view: ntt_loop_lvls)
+    // returns (y': seq<elem>)
+    //     requires view.ntt_level_loop_inv(y);
+    //     requires view.ki < chunk_count(view.higher.m);
+    //     requires k == view.hi_idx() * view.higher.m.full;
+    // {
+    //     y' := y;
+    //     var len' := view.lower.m;
+    //     var omgm := omega_n(view.higher.m);
+
+    //     var omg := 1;
+    //     var j := 0;
+
+    //     assert omg == modpow(omgm, 0) by {
+    //         LemmaPow0Auto();
+    //     }
+
+    //     pow2_basics(view.higher.m);
+
+    //     view.index_bounded_lemma(0);
+    //     view.index_bounded_lemma(len'.full);
+
+    //     view.lower_view_correspondence(y, k);
+    //     // ghost var even_chunk := read_chunk(y, view.lower.m, view.lo_idx());
+    //     // ghost var odd_chunk := read_chunk(y, view.lower.m, view.lo_idx()+1);
+        
+    //     // view.hi_lo_idx_relations();
+    //     // assert y'[k+j..k+len'.full] == even_chunk;
+
+    //     while (j < len'.full)
+    //         invariant 0 <= j <= len'.full;
+    //         invariant omg == modpow(omgm, j);
+    //         invariant |y'| == |y|;
+    //         invariant k + j + len'.full <= N;
+    //         invariant y'[..k] == y[..k];
+    //         invariant y'[k+j..k+len'.full] == y[k+j..k+len'.full];
+    //         invariant y'[k+len'.full+j..] == y[k+len'.full+j..];
+    //     {
+    //         view.index_bounded_lemma(j);
+
+    //         var t := modmul(omg, y[k + j + len'.full]);
+    //         var u := y[k + j];
+    //         y' := y'[k + j := modadd(u, t)];
+    //         y' := y'[k + j + len'.full := modsub(u, t)];
+
+    //         omg_inv(omgm, omg, view.higher.m, j);
+    //         omg := modmul(omg, omgm);
+    //         j := j + 1;
+    //     }
+
+    //     // assert y[..k] == y'[..k];
+    //     // assert y[k+m.full..] == y'[k+m.full..];
+    // }
 
 
     // method ntt_level_loop(a: seq<elem>, s: nat)
@@ -279,7 +333,7 @@ module ntt {
     //     }
     // }
 
-    // method ntt(b: seq<elem>, len: pow2_t) returns (y: seq<elem>)
+    // method ntt(b: seq<elem>, len: pow2_t) returns (y: n_sized)
     //     requires |b | == len.full == N;
     //     requires len.exp == L;
     //     // ensures poly_eval_all_points(a, y, len)
@@ -296,7 +350,7 @@ module ntt {
 
 
       // lemma init_implies_inv(
-    //     y: seq<elem>,
+    //     y: n_sized,
     //     m: pow2_t, 
     //     a: seq<seq<elem>>,
     //     idxs: seq<seq<index_t>>)
@@ -306,9 +360,9 @@ module ntt {
     //     requires 0 == m.exp;
     //     requires ntt_chunk_indicies_inv(a, idxs, m);
     //     requires y == Ar();
-    //     ensures ntt_chunk_loop_inv(y, m, a, idxs);
+    //     ensures ntt_level_loop_inv(y, m, a, idxs);
     // {
-    //     var view := view_as_chunks(y, m);
+    //     var view := y_as_chunks(y, m);
     //     var base := ntt_rec3_base(a, m, idxs);
     //     forall ki | 0 <= ki < N
     //         ensures view[ki] == base[ki];
@@ -324,3 +378,96 @@ module ntt {
     // }
 }
 
+
+
+
+    // function {:opaque} y_as_chunks_prefix(y: n_sized, len: pow2_t, i: nat): seq<seq<elem>>
+    //     requires 0 <= len.exp <= L;
+    //     requires i <= chunk_count(len);
+    // {
+    //     var count := i;
+    //     var csize := len.full;
+    //     chunk_index_bounded_auto(len);
+    //     seq(count, ki requires 0 <= ki < count => y[ki * csize..ki * csize + csize])    
+    // }
+
+    // lemma y_as_chunks_prefix_lemma(y: n_sized, y': n_sized, len: pow2_t, i: nat)
+    //     requires 0 <= len.exp <= L;
+    //     requires i <= chunk_count(len);
+    //     requires 0 <= i * len.full <= N;
+    //     requires y[..i * len.full] == y'[..i * len.full];
+    //     ensures y_as_chunks_prefix(y, len, i) == y_as_chunks_prefix(y', len, i);
+    // {
+    //     reveal y_as_chunks_prefix();
+    //     var csize := len.full;
+    //     var v1 := y_as_chunks_prefix(y, len, i);
+    //     var v2 := y_as_chunks_prefix(y', len, i);
+
+    //     forall ki: nat | 0 <= ki < i
+    //         ensures v1[ki] == v2[ki];
+    //     {
+    //         chunk_index_bounded(len, ki);
+
+    //         var lo := ki * csize;
+    //         var hi := ki * csize + csize;
+
+    //         assert hi <= i * len.full by {
+    //             LemmaMulInequality(ki, i-1, len.full);
+    //             LemmaMulIsCommutativeAuto();
+    //             LemmaMulIsDistributiveSubAuto();
+    //         }
+
+    //         assert y[..hi] == y'[..hi];
+    //         assert y[lo..hi] == y'[lo..hi];
+
+    //     }
+    // }
+
+    // function {:opaque} y_as_chunks_suffix(y: n_sized, len: pow2_t, i: nat): seq<seq<elem>>
+    //     requires 0 <= len.exp <= L;
+    //     requires i <= chunk_count(len);
+    // {
+    //     var count := chunk_count(len) - i;
+    //     var csize := len.full;
+        
+    //     assert forall ki | 0 <= ki < count ::
+    //         0 <= (ki + i) * csize <= N - csize by {
+    //         forall ki | 0 <= ki < count 
+    //             ensures 0 <= (ki + i) * csize <= N - csize;
+    //         {
+    //             chunk_index_bounded(len, ki + i);
+    //         }
+    //     }
+    //     seq(count, ki requires 0 <= ki < count => y[(ki + i) * csize..(ki + i) * csize + csize]) 
+    // }
+
+    // lemma y_as_chunks_suffix_lemma(y: n_sized, y': n_sized, len: pow2_t, i: nat)
+    //     requires 0 <= len.exp <= L;
+    //     requires i <= chunk_count(len);
+    //     requires 0 <= i * len.full <= N;
+    //     requires y[i * len.full..] == y'[i * len.full..];
+    //     ensures y_as_chunks_suffix(y, len, i) == y_as_chunks_suffix(y', len, i);
+    // {
+    //     reveal y_as_chunks_suffix();
+    //     var count := chunk_count(len) - i;
+    //     var csize := len.full;
+    //     var v1 := y_as_chunks_suffix(y, len, i);
+    //     var v2 := y_as_chunks_suffix(y', len, i);
+
+    //     forall ki: nat | 0 <= ki < count
+    //         ensures v1[ki] == v2[ki];
+    //     {
+    //         chunk_index_bounded(len, ki + i);
+
+    //         var lo := (ki + i) * csize;
+    //         var hi := lo + csize;
+
+    //         assert i * len.full <= lo by {
+    //             assert i <= ki + i;
+    //             LemmaMulInequality(i, i+ki, len.full);
+    //         }
+
+    //         assert y[lo..] == y'[lo..];
+    //         assert y[lo..hi] == y'[lo..hi];
+    //     }
+    // }
