crypto_examples/ntt_rec3.dfy
@@ -23,12 +23,6 @@ module ntt_recs3 {
         ensures chunk_count(pow2_half(m)) == chunk_count(m) * 2;
     {
         assume false; // TODO
-        // nth_root_lemma();
-        // var m' := pow2_half(m);
-        // var count := chunk_count(m);
-        // assert count == N / m.full;
-        // var count' := chunk_count(m');
-        // assert count' == N / m'.full;
     }
 
     datatype level_view = level_cons(
@@ -75,6 +69,7 @@ module ntt_recs3 {
 
         function method ntt_rec3(): (ys: seq<seq<elem>>)
             requires valid_level_view()
+            ensures level_eval(ys)
             decreases m.exp;
         {
             pow2_basics(m);
